userbase example

example_userbase.thy
@@ -2,12 +2,35 @@ theory example_userbase
 imports approach
 begin
 
+
+definition 
+"i_callOriginI ctxt c \<equiv> 
+  case i_callOrigin ctxt c of Some t \<Rightarrow> i_transactionOrigin ctxt t | None \<Rightarrow> None"
+
+text {* lifting the happensBefore relation on database-calls to the level of invocations. *}
+definition 
+"invocation_happensBefore ctxt \<equiv> 
+  {(x,y). (\<exists>c. i_callOriginI ctxt c \<triangleq> x) 
+        \<and> (\<exists>c. i_callOriginI ctxt c \<triangleq> y) 
+        \<and> (\<forall>cx cy. i_callOriginI ctxt cx \<triangleq> x
+                 \<and> i_callOriginI ctxt cy \<triangleq> y
+                 \<longrightarrow> (cx,cy)\<in>happensBefore ctxt)}"
+
+
+(* ^^^^ *)
+
 datatype val =
     String string
   | UserId int
   | Bool bool
   | Undef
+  | Found string string
+  | NotFound
 
+fun stringval where
+  "stringval (String s) = s"
+| "stringval _ = ''''"
+  
 record localState = 
   ls_pc :: nat
   ls_u :: val
@@ -15,8 +38,8 @@ record localState =
   ls_mail :: string
   ls_exists :: bool
 
-definition initialState :: "localState" where
-"initialState = \<lparr>
+definition lsInit :: "localState" where
+"lsInit = \<lparr>
   ls_pc = 0,
   ls_u = Undef,
   ls_name = '''',
@@ -50,24 +73,125 @@ definition updateMailImpl :: "(localState, val) procedureImpl" where
    (* 6 *) Return Undef
    ] ! ls_pc ls"   
    
+definition removeUserImpl :: "(localState, val) procedureImpl" where
+"removeUserImpl ls \<equiv> [
+   (* 0 *) BeginAtomic (ls\<lparr>ls_pc := 1\<rparr>),
+   (* 1 *) DbOperation ''users_remove'' [ls_u ls] (\<lambda>r. ls\<lparr>ls_pc := 2 \<rparr>),
+   (* 2 *) EndAtomic  (ls\<lparr>ls_pc := 3\<rparr>),
+   (* 3 *) Return Undef
+   ] ! ls_pc ls"      
+   
+definition getUserImpl :: "(localState, val) procedureImpl" where
+"getUserImpl ls \<equiv> [
+   (* 0 *) BeginAtomic (ls\<lparr>ls_pc := 1\<rparr>),
+   (* 1 *) DbOperation ''users_contains_key'' [ls_u ls] (\<lambda>r. ls\<lparr>ls_exists := (r = Bool True), ls_pc := 2 \<rparr>),
+   (* 2 *) LocalStep (if ls_exists ls then ls\<lparr>ls_pc := 3\<rparr> else ls\<lparr>ls_pc := 5\<rparr> ),
+   (* 3 *) DbOperation ''users_name_get'' [ls_u ls] (\<lambda>r. ls\<lparr>ls_name := stringval r, ls_pc := 4 \<rparr>),
+   (* 4 *) DbOperation ''users_mail_get'' [ls_u ls] (\<lambda>r. ls\<lparr>ls_mail := stringval r, ls_pc := 5 \<rparr>),
+   (* 5 *) EndAtomic  (ls\<lparr>ls_pc := 6\<rparr>),
+   (* 6 *) Return (if ls_exists ls then Found (ls_name ls) (ls_mail ls) else NotFound )
+   ] ! ls_pc ls"      
+   
+   
 definition procedures where
 "procedures proc args \<equiv> 
   if proc = ''registerUser'' then
     case args of 
       [String name, String mail] \<Rightarrow> 
-        Some (initialState\<lparr>ls_name := name, ls_mail := mail \<rparr> , registerUserImpl)
+        Some (lsInit\<lparr>ls_name := name, ls_mail := mail \<rparr> , registerUserImpl)
       | _ \<Rightarrow> None
+  else if proc = ''updateMail'' then 
+    case args of 
+      [UserId u, String mail] \<Rightarrow> 
+        Some (lsInit\<lparr>ls_u := UserId u, ls_mail := mail \<rparr> , updateMailImpl)
+      | _ \<Rightarrow> None
+  else if proc = ''removeUser'' then 
+    case args of 
+      [UserId u] \<Rightarrow> 
+        Some (lsInit\<lparr>ls_u := UserId u \<rparr> , removeUserImpl)
+      | _ \<Rightarrow> None
+  else if proc = ''getUser'' then 
+    case args of 
+      [UserId u] \<Rightarrow> 
+        Some (lsInit\<lparr>ls_u := UserId u \<rparr> , getUserImpl)
+      | _ \<Rightarrow> None  
   else 
     None"
 
-    
-    
+
+definition latest_name_assign :: "val operationContext \<Rightarrow> val \<Rightarrow> val set" where
+"latest_name_assign ctxt u \<equiv>  {v | c1 v. 
+     calls ctxt c1 \<triangleq> Call ''users_name_assign'' [u, v] Undef
+   \<and> (\<forall>c2. calls ctxt c2 \<triangleq> Call ''users_remove'' [u] Undef \<longrightarrow> (c2,c1)\<in>happensBefore ctxt)
+   \<and> (\<forall>c2 v'. calls ctxt c2 \<triangleq> Call ''users_name_assign'' [u] v' \<longrightarrow> \<not>(c1,c2)\<in>happensBefore ctxt)}"
+
+definition latest_mail_assign :: "val operationContext \<Rightarrow> val \<Rightarrow> val set" where
+"latest_mail_assign ctxt u \<equiv>  {v | c1 v. 
+     calls ctxt c1 \<triangleq> Call ''users_mail_assign'' [u, v] Undef
+   \<and> (\<forall>c2. calls ctxt c2 \<triangleq> Call ''users_remove'' [u] Undef \<longrightarrow> (c2,c1)\<in>happensBefore ctxt)
+   \<and> (\<forall>c2 v'. calls ctxt c2 \<triangleq> Call ''users_mail_assign'' [u] v' \<longrightarrow> \<not>(c1,c2)\<in>happensBefore ctxt)}"   
+   
+definition crdtSpec :: "operation \<Rightarrow> val list \<Rightarrow> val operationContext \<Rightarrow> val \<Rightarrow> bool" where
+"crdtSpec oper args ctxt res \<equiv> 
+  if oper \<in> {''users_name_assign'', ''users_mail_assign'', ''users_remove''} then
+    (* update-operations always return Undef *)
+    res = Undef
+  else if oper = ''users_contains_key'' then
+    res = Bool (\<exists>c1 v. (calls ctxt c1 \<triangleq> Call ''users_name_assign'' (args @ [v]) Undef
+                 \<or> calls ctxt c1 \<triangleq> Call ''users_mail_assign'' (args @ [v]) Undef)
+               \<and> (\<forall>c2. calls ctxt c2 \<triangleq> Call ''users_remove'' args Undef \<longrightarrow> (c2,c1)\<in>happensBefore ctxt))
+  else if oper = ''users_name_get'' then 
+    if latest_name_assign ctxt (hd args) = {} then 
+      res = Undef
+    else
+      res \<in> latest_name_assign ctxt (hd args)
+  else if oper = ''users_mail_get'' then 
+    if latest_mail_assign ctxt (hd args) = {} then 
+      res = Undef
+    else
+      res \<in> latest_mail_assign ctxt (hd args)
+  else
+    False"
+  
+definition inv1 :: "val invariantContext \<Rightarrow> bool" where
+"inv1 ctxt \<equiv> \<forall>r g u.
+    i_invocationOp ctxt r \<triangleq> (''removeUser'', [u])
+  \<and> i_invocationOp ctxt g \<triangleq> (''getUser'', [u])
+  \<and> (r,g) \<in> invocation_happensBefore ctxt
+  \<longrightarrow> i_invocationRes ctxt g \<triangleq> NotFound"
+  
+definition inv2 :: "val invariantContext \<Rightarrow> bool" where
+"inv2 ctxt \<equiv> \<forall>u i.
+    i_invocationOp ctxt i \<triangleq> (''removeUser'', [u])
+  \<and> i_invocationRes ctxt i \<noteq> None
+  \<longrightarrow> (\<exists>c. i_callOriginI ctxt c \<triangleq> i \<and> calls ctxt c \<triangleq> Call ''users_remove'' [u] Undef)"
+  
+definition inv3 :: "val invariantContext \<Rightarrow> bool" where
+"inv3 ctxt \<equiv> \<not>(\<exists>write delete u v.
+  (calls ctxt write \<triangleq> Call ''users_name_assign'' [u, v] Undef
+    \<or> calls ctxt write \<triangleq> Call ''users_mail_assign'' [u, v] Undef)
+  \<and> (calls ctxt delete \<triangleq> Call ''users_remove'' [u] Undef)
+  \<and> (delete, write) \<in> happensBefore ctxt
+  )"
+  
+definition inv :: "val invariantContext \<Rightarrow> bool" where
+"inv ctxt \<equiv> inv1 ctxt \<and> inv2 ctxt \<and> inv3 ctxt"
+  
 definition prog :: "(localState, val) prog" where
 "prog \<equiv> \<lparr>
-  querySpec = ???,
+  querySpec = crdtSpec,
   procedure = procedures,
-  invariant = ???
+  invariant = inv
 \<rparr>"
+
+theorem "programCorrect prog"
+proof (rule show_correctness_via_single_session)
+  show "invariant_all (replissSem1.initialState prog)"
+     by (auto simp add: initialState_def invariant_all_def prog_def inv_def inv1_def inv2_def inv3_def invContextH_def)
+  
+  show "programCorrect_s example_userbase.prog"
+  apply (auto simp add: programCorrect_s_def)
+  apply (auto simp add: prog_def step_s.simps)
 
 
 
